fnish proofs

examples/layeredeffects/AlgForAll.fst
@@ -9,12 +9,11 @@ module W = FStar.WellFounded
 module T = FStar.Tactics
 open LatticeAlg
 
-
 let pre = state -> Type0
 let post (a:Type) = a -> state -> Type0
 let st_wp (a:Type) : Type = post a -> pre
 
-let return_wp #a x : st_wp a = fun p s -> p x s 
+let return_wp #a x : st_wp a = fun p s -> p x s
 
 let bind_wp #a #b (w : st_wp a) (wf : a -> st_wp b)
   : st_wp b
@@ -31,8 +30,8 @@ let rec interp_as_wp #a (t : repr a [Read;Write]) : st_wp a =
   | Act Read _ k ->
     bind_wp read_wp (fun s -> WF.axiom1 k s; interp_as_wp (k s))
   | Act Write s k ->
-    bind_wp (write_wp s) (fun () -> WF.axiom1 k (); interp_as_wp (k ()))
-  
+    bind_wp (write_wp s) (fun (o:unit) -> WF.axiom1 k o; interp_as_wp (k o))
+
 // m is a monad.
 val m (a : Type u#a) : Type u#a
 let m a = repr a [Read;Write]
@@ -52,18 +51,12 @@ let w_return = return_wp
 val w_bind (#a #b : Type) : w a -> (a -> w b) -> w b
 let w_bind = bind_wp
 
-val stronger : (#a:Type) -> FStar.Preorder.preorder (w a)
+(* Bug: defining this as a FStar.Preorder.preorder
+causes stupid failures ahead *)
+val stronger : (#a:Type) -> w a -> w a -> Type0
 let stronger w1 w2 = forall p s. w1 p s ==> w2 p s
 
 let equiv #a (w1 w2 : w a) = w1 `stronger` w2 /\ w2 `stronger` w1
-
-let bind_is_monotonic
-  (#a #b : Type)
-  (w1 w2 : w a) 
-  (f1 f2 : a -> w b)
-  : Lemma (requires (w1 `stronger` w2 /\ (forall x. f1 x `stronger` f2 x)))
-          (ensures (w_bind w1 f1 `stronger` w_bind w2 f2))
-  = admit ()
 
 let (<<=) = stronger
 
@@ -75,15 +68,80 @@ val interp_ret (#a:Type) (x:a)
   : Lemma (interp (m_return x) `equiv` w_return x)
 let interp_ret x = assert (interp (m_return x) `equiv` w_return x) by (T.compute ())
 
+let wp_is_monotonic #a (wp : w a) : Type0 =
+  forall p1 p2 s0. (forall x s1. p1 x s1 ==> p2 x s1) ==> wp p1 s0 ==> wp p2 s0
+
+let bind_preserves_mon #a #b (wp : w a) (f : a -> w b)
+  : Lemma (requires (wp_is_monotonic wp /\ (forall x. wp_is_monotonic (f x))))
+          (ensures (wp_is_monotonic (bind_wp wp f)))
+  = ()
+
+let rec interp_monotonic #a (c:m a) : Lemma (wp_is_monotonic (interp c)) =
+  match c with
+  | Return x -> ()
+  | Act Read _ k ->
+    let aux (x:state) : Lemma (wp_is_monotonic (interp (k x))) =
+      WF.axiom1 k x;
+      interp_monotonic (k x)
+    in
+    Classical.forall_intro aux;
+    bind_preserves_mon read_wp (fun x -> interp (k x))
+  | Act Write s k ->
+    let aux (x:unit) : Lemma (wp_is_monotonic (interp (k x))) =
+      WF.axiom1 k x;
+      interp_monotonic (k x)
+    in
+    Classical.forall_intro aux;
+    bind_preserves_mon (write_wp s) (fun x -> interp (k x))
+
+let elim_str #a (w1 w2 : w a) (p : post a) (s0:state)
+  : Lemma (requires (w1 <<= w2))
+          (ensures w1 p s0 ==> w2 p s0)
+  = ()
+
+let rec interp_morph #a #b (c : m a) (f : a -> m b) (p:_) (s0:_)
+  : Lemma (interp c (fun y s1 -> interp (f y) p s1) s0 == interp (m_bind c f) p s0)
+  = match c with
+    | Return x -> ()
+    | Act Read _ k ->
+      let aux (o:state) : Lemma (interp (k o) (fun y s1 -> interp (f y) p s1) s0
+                                        == interp (m_bind (k o) f) p s0) =
+        WF.axiom1 k o;
+        interp_morph (k o) f p s0
+      in
+      Classical.forall_intro aux
+
+    | Act Write s k ->
+      let aux (o:unit) : Lemma (interp (k o) (fun y s1 -> interp (f y) p s1) s
+                                        == interp (m_bind (k o) f) p s) =
+        WF.axiom1 k o;
+        interp_morph (k o) f p s
+      in
+      Classical.forall_intro aux
+
+    | _ ->
+      unreachable ()
+
 val interp_bind (#a #b:Type)
   (c : m a) (f : a -> m b)
-  : Lemma (interp (m_bind c f) `equiv` w_bind (interp c) (fun x -> interp (f x)))
-let interp_bind c f =
-  calc equiv {
-    interp (m_bind c f);
-    equiv { admit() }
-    w_bind (interp c) (fun x -> interp (f x));
-  }
+  (w1 : w a) (w2 : a -> w b)
+  : Lemma (requires w1 <<= interp c /\ (forall x. w2 x <<= interp (f x)))
+          (ensures w_bind w1 w2 `stronger` interp (m_bind c f))
+let interp_bind #a #b c f w1 w2 =
+  let aux (p:post b) (s0:state) : Lemma (w_bind w1 w2 p s0 ==> interp (m_bind c f) p s0) =
+    calc (==>) {
+      w_bind w1 w2 p s0;
+      ==> {}
+      w1 (fun y s1 -> w2 y p s1) s0;
+      ==> { (* hyp *)}
+      interp c (fun y s1 -> w2 y p s1) s0;
+      ==> { interp_monotonic c }
+      interp c (fun y s1 -> interp (f y) p s1) s0;
+      ==> { interp_morph c f p s0 }
+      interp (m_bind c f) p s0;
+    }
+  in
+  Classical.forall_intro_2 aux
 
 let repr (a : Type) (w: w a) = c:(m a){w `stronger` interp c}
 
@@ -95,17 +153,9 @@ let bind (a : Type) (b : Type)
   (wp_v : w a) (wp_f: a -> w b)
   (v : repr a wp_v) (f : (x:a -> repr b (wp_f x)))
   : repr b (w_bind wp_v wp_f) =
-  let r = m_bind v f in
-  (* Proof that stronger holds *)
-  calc (<<=) {
-    w_bind wp_v wp_f;
-    <<= { bind_is_monotonic wp_v (interp v) wp_f (fun x -> interp (f x)) (* from the refinement *) }
-    w_bind (interp v) (fun x -> interp (f x));
-    <<= { interp_bind v f }
-    interp (m_bind v f);
-  };
-  r
-  
+  interp_bind v f wp_v wp_f;
+  m_bind v f
+
 let subcomp (a:Type) (w1 w2: w a)
   (f : repr a w1)
   : Pure (repr a w2)
@@ -124,7 +174,7 @@ layered_effect {
   with repr         = repr;
        return       = return;
        bind         = bind;
-       subcomp      = subcomp; 
+       subcomp      = subcomp;
        if_then_else = if_then_else
 }
 
@@ -136,7 +186,7 @@ let _get : repr state read_wp =
 
 let get () : DM4A state read_wp =
   DM4A?.reflect _get
-  
+
 let _put (s:state) : repr unit (write_wp s) =
   let c0 : LatticeAlg.repr unit [Read;Write] = LatticeAlg._put s in
   let w = interp_as_wp c0 in
@@ -148,12 +198,12 @@ let put (s:state) : DM4A unit (write_wp s) =
 
 let lift_pure_wp (#a:Type) (wp : pure_wp a) : st_wp a =
   fun p s0 -> wp (fun x -> p x s0)
- 
+
 let lift_pure_dm4a (a:Type) wp (f:(eqtype_as_type unit -> PURE a wp))
   : Pure (repr a (lift_pure_wp wp)) // can't call f() here, so lift its wp instead
          (requires (wp (fun _ -> True)))
          (ensures (fun _ -> True))
-  = 
+  =
     let v : a = elim_pure f (fun _ -> True) in
     FStar.Monotonic.Pure.wp_monotonic_pure ();
     assert (forall p. wp p ==> p v); // this is key fact needed for the proof
@@ -161,9 +211,6 @@ let lift_pure_dm4a (a:Type) wp (f:(eqtype_as_type unit -> PURE a wp))
     Return v
 
 sub_effect PURE ~> DM4A = lift_pure_dm4a
-
-[@@expect_failure] // lift doesn't really work
-let test () : DM4A int (w_return 5) = r 5
 
 let addx (x:int) : DM4A unit (fun p s0 -> p () (s0+x)) by (T.norm [delta]) =
   let y = get () in
